src/frontends/lean/token_table.h
@@ -17,7 +17,7 @@ Author: Leonardo de Moura
 namespace lean {
 // User-level maximum precedence
 unsigned get_max_prec();
-// Internal maximum precedence used for @@, @ and ! operators
+// Internal maximum precedence used for @@ and @ operators
 unsigned get_Max_prec();
 unsigned get_arrow_prec();
 class token_info {
