tests/lean/run/auto_propext.lean
@@ -2,4 +2,4 @@ example (p q : Prop) (h : p) : q ∨ p :=
 by simp [h]
 
 example (p q : Prop) : p → q ∨ p :=
-by ctx_simp
+by simp {contextual := tt}
